src/Employees/Implementation/VAPoda2.dfy
@@ -90,23 +90,7 @@ method {:only} Cota(ps : Solution, input : Input, min : real) returns (cota : re
                             && s.Valid(input.Model())
     ensures s.TotalTime(input.Model().times) >= cota
   {
-
-    assert ps.totalTime == ps.Model().TotalTime(input.Model().times);
-
-    var diferencia := s.TotalTime(input.Model().times) - ps.totalTime;
-
-    assert s.TotalTime(input.Model().times) >= ps.totalTime + (rest * min) by {
-      assert ps.totalTime == ps.Model().TotalTime(input.Model().times);
-      assert s.Extends(ps.Model());
-      assert input.IsMin(min, 0);
-      ps.Model().GreaterOrEqualTimeFromExtends(s, input.Model());
-      assert s.TotalTime(input.Model().times) >= ps.totalTime;
-      assert forall i | 0 <= i < ps.k :: min <= input.times[i, ps.Model().employeesAssign[i]];
-      var s' := SolutionData(s.employeesAssign, ps.k);
-      //assert s'.TotalTime(input.Model().times) == ps.totalTime;
-      assert forall i | ps.k <= i < |s.employeesAssign| :: min <= input.times[i, s.employeesAssign[i]];
-      assume diferencia >= (rest * min);
-    }
+    SolutionData.AddTimesLowerBound(ps.Model(),s,input.Model(),min);   
   }
 }
 
